Cleanup categories

theories/Category.v
@@ -8,146 +8,135 @@ Require Blech.Map.
 
 Import IfNotations.
 
-(*
- Maps are behaviour preserving transformations between terms.  This
- way we get identity and composition for free without finicky
- substitution issues.
- *)
 Module Import Hor.
   (* FIXME preserve behaviour as well *)
-  Class Hor (A B: type) f := {
-      preserves_types {Γ v}: Γ ⊢ v in A -> Γ ⊢ f v in B ;
-  }.
+  Definition Hor (A B: type) v :=
+    Map.one 0 A ⊢ v in B.
+  Existing Class Hor.
 
-  Definition id x: term := x.
+  Definition id: term := v_var 0.
   Instance id_Hor A: Hor A A id.
   Proof using.
-    exists.
-    auto.
+    unfold Hor.
+    constructor.
+    cbn.
+    reflexivity.
   Defined.
 
-  Definition compose (f g: term -> term) x := f (g x).
+  Definition compose f g := subst_term g 0 f.
   Instance compose_Hor f g {A B C} `{Hor B C f} `{Hor A B g}: Hor A C (compose f g).
   Proof.
-    exists.
-    intros.
-    unfold compose.
-    apply preserves_types.
-    apply preserves_types.
-    auto.
+    unfold Hor in *.
+    generalize dependent C.
+    generalize dependent B.
+    generalize dependent A.
+    generalize dependent g.
+    induction f.
+    all: cbn.
+    all: intros g A B p C q.
+    - destruct (eq_var x 0).
+      + subst.
+        inversion q.
+        subst.
+        unfold Map.one in H1.
+        rewrite Map.find_add in H1.
+        inversion H1.
+        subst.
+        auto.
+      + inversion q.
+        subst.
+        rewrite Map.find_one_ne in H1.
+        1: discriminate.
+        auto.
+    - inversion q.
+      subst.
+      constructor.
+    - inversion q.
+      subst.
+      econstructor.
+      eapply IHf.
+      all: eauto.
+    - inversion q.
+      subst.
+      econstructor.
+      eapply IHf.
+      all: eauto.
+    - inversion q.
+      subst.
+      econstructor.
+      all: try eapply IHf1 ; try eapply IHf2.
+      all: eauto.
   Defined.
 
-  Definition tt (x: term) := v_tt.
-  Instance tt_Hor A: Hor A t_unit tt.
+  Instance tt_Hor A: Hor A t_unit v_tt.
   Proof.
-    exists.
-    intros.
     constructor.
   Defined.
 
-  Definition fanout (f g: term -> term) x := v_fanout (f x) (g x).
-  Instance fanout_Hor f g {A B C} `{Hor C A f} `{Hor C B g}: Hor C (t_prod A B) (fanout f g).
+  Instance fanout_Hor f g {A B C} `{Hor C A f} `{Hor C B g}: Hor C (A * B) (v_fanout f g).
   Proof.
-    exists.
-    intros.
-    unfold fanout.
     constructor.
-    all: apply preserves_types.
     all: auto.
   Defined.
 
-  Instance fst_Hor A B : Hor (t_prod A B) A v_fst.
+  Instance fst_Hor A B : Hor (A * B) A (v_fst (v_var 0)).
   Proof.
-    exists.
-    intros.
     econstructor.
-    eauto.
+    constructor.
+    cbn.
+    reflexivity.
   Defined.
 
-  Instance snd_Hor A B : Hor (t_prod A B) B v_snd.
+  Instance snd_Hor A B : Hor (A * B) B (v_snd (v_var 0)).
   Proof.
-    exists.
-    intros.
     econstructor.
-    eauto.
+    constructor.
+    cbn.
+    reflexivity.
   Defined.
 
   (* FIXME define setoid equality and prove laws *)
-
-  Section Subst.
-    Variable X: var.
-
-    Definition to (v: term) (v': term) := subst_term v' X v.
-    Definition from (f: term -> term) := f (v_var X).
-
-    Instance to_Hor v A B: Map.one X A ⊢ v in B -> Hor A B (to v).
-    Proof.
-      unfold to.
-      generalize dependent B.
-      generalize dependent A.
-      induction v.
-      all: intros A B p.
-      all: cbn.
-      all: constructor.
-      all: intros Γ v' q.
-      - destruct (eq_var x X).
-        + subst.
-          inversion p.
-          subst.
-          unfold Map.one in H1.
-          rewrite Map.find_add in H1.
-          inversion H1.
-          subst.
-          auto.
-        + inversion p.
-          subst.
-          rewrite Map.find_one_ne in H1.
-          1: discriminate.
-          auto.
-      - inversion p.
-        subst.
-        constructor.
-      - inversion p.
-        subst.
-        econstructor.
-        apply (@preserves_types _ _ _ (IHv _ _ X0)).
-        eauto.
-      - inversion p.
-        subst.
-        econstructor.
-        apply (@preserves_types _ _ _ (IHv _ _ X0)).
-        auto.
-      - inversion p.
-        subst.
-        econstructor.
-        + apply (@preserves_types _ _ _ (IHv1 _ _ X0)).
-          auto.
-        + apply (@preserves_types _ _ _ (IHv2 _ _ X1)).
-          auto.
-    Defined.
-    End Subst.
 End Hor.
 
 Module Import Vert.
-  Class Vert (A B: type) f := {
-      preserves_types {Γ E}: Γ ⊢ E ? A -> Γ ⊢ f E ? B ;
-  }.
+  Definition Vert (A B: type) f :=
+    Map.empty ⊢ f ? A * B.
+  Existing Class Vert.
 
-  Definition id x: context := x.
-  Instance id_Vert A: Vert A A id.
+  Definition id A := E_lam 0 A (E_var 0).
+  Instance id_Vert A: Vert A A (id A).
   Proof using.
-    exists.
-    auto.
+    unfold Vert.
+    apply (Context.typecheck_sound Map.empty).
+    cbn.
+    destruct (Context.eq_type A A).
+    2: contradiction.
+    cbn.
+    unfold Map.one.
+    rewrite Map.minus_add.
+    reflexivity.
   Defined.
 
-  Definition compose (f g: context -> context) x := f (g x).
-  Instance compose_Vert f g {A B C} `{Vert B C f} `{Vert A B g}: Vert A C (compose f g).
+  Definition compose (f g: context) A := E_lam 0 A (E_app f (E_app g (E_var 0))).
+  Instance compose_Vert f g {A B C} `{Vert B C f} `{Vert A B g}: Vert A C (compose f g A).
   Proof.
-    exists.
-    intros.
+    unfold Vert in *.
     unfold compose.
-    apply preserves_types.
-    apply preserves_types.
-    auto.
+    constructor.
+    replace (Map.add 0 A _) with (Map.merge Map.empty (Map.one 0 A)).
+    2: {
+      rewrite Map.merge_empty_l.
+      reflexivity.
+    }
+    econstructor.
+    1: eauto.
+    replace (Map.one 0 A) with (Map.merge Map.empty (Map.one 0 A)).
+    2: {
+      rewrite Map.merge_empty_l.
+      reflexivity.
+    }
+    econstructor.
+    1: eauto.
+    constructor.
   Defined.
 End Vert.
